mac format rpc example ready for the tutorial

examples/unit-tests/mac.fst
@@ -18,27 +18,38 @@
    hashes, namely HMAC-SHA1, and their idealization under the INT-CMA
    computational assumption *)
 
-module MAC 
-
+module SHA1 
 open Array
+
 type bytes = seq byte (* concrete byte arrays *) 
 type text  = bytes    (* a type abbreviation, for clarity *)
 
-type nbytes (n:nat) = b:bytes{length b == n} (* fixed-length bytes *)
-
-let keysize = 16 (* these are the sizes for SHA1 *) 
-let macsize = 20  
-type key = nbytes keysize
-type tag = nbytes macsize
+type nbytes (n:nat) = 
+  b:bytes{length b == n} (* fixed-length bytes *)
 
 (* we rely on some external crypto library implementing HMAC-SHA1 *)
 
+let keysize = 16 
+let macsize = 20  
+
+type key = nbytes keysize
+type tag = nbytes macsize
+
+assume val sample: n:nat -> nbytes n
 assume val sha1: key -> text -> Tot tag 
+
 
 (* to verify, we simply recompute & compare *) 
 
 val sha1verify: key -> text -> tag -> Tot bool
 let sha1verify k txt tag = (sha1 k txt = tag)
+
+
+module MAC 
+open Array
+open SHA1
+
+(* ---- specification *)
 
 (* we attach an authenticated properties to each key, 
    used as a pre-condition for MACing and 
@@ -47,29 +58,26 @@ let sha1verify k txt tag = (sha1 k txt = tag)
 opaque type key_prop : key -> text -> Type
 type pkey (p:(text -> Type)) = k:key{key_prop k == p}
 
-assume val keygen: p:(text -> Type) -> pkey p
-
+val keygen: p:(text -> Type) -> pkey p
 val mac:    k:key -> t:text{key_prop k t} -> tag
 val verify: k:key -> t:text -> tag -> b:bool{b ==> key_prop k t}
 
-(* to model authentication, we log all genuine calls to MACs *) 
+(* ---- implementation *)
 
-(* the ideal implementation below uses a global log *)
+let keygen (p: (text -> Type)) = 
+  let k = sample keysize in
+  assume (key_prop k == p);
+  k
 
-(* TODO Can we use a constructor instead of an attached property? *)
-(* TODO make keys abstract except within this module *) 
-
-(* TODO provide a concrete implementation of keygen, aka sample 16
-   random bytes + maybe a counter it would be better to avoid assuming
-   key_prop; see also encrypt.fst *)
+(* to model authentication, we log all genuine calls 
+   to MACs; the ideal implementation below uses the 
+   log to correct errors. *)
 
 type entry = 
-  | Entry : k:key
+  | Entry : k:key 
          -> t:text{key_prop k t}
          -> m:tag
          -> entry
-
-(* TODO why assumed? we miss toplevel side effects... *) 
 
 let log = ST.alloc (list entry) [] 
 
@@ -78,14 +86,13 @@ let mac k t =
   log := Entry k t m :: !log;
   m
 
-(*
-val filter:  k:key -> t:text -> s:tag -> e:entry -> b: bool { b ==> e = Entry k t s }
-let filter k text tag (Entry k' text' tag') = k=k' && text=text' (*CTXT: && tag=tag' *) 
- *)
-
 let verify k text tag =
   let verified = sha1verify k text tag in 
-  let found =  is_Some (List.find (function (Entry k' text' tag') -> k=k' && text=text' (*CTXT: && tag=tag' *) ) !log) in 
+  let found =
+    is_Some 
+      (List.find 
+        (fun (Entry k' text' tag') -> k=k' && text=text')
+        !log) in 
 
   (* plain, concrete implementation (ignoring the log) *) 
 //verified           
@@ -97,5 +104,8 @@ let verify k text tag =
 //(if verified && not found then win := Some(k,text,tag)); 
 //verified
 
+
 (* VARIANT CTXT vs CPA: is the tag authenticated?
    otherwise do not include m:tag in the entry *)
+
+//      (fun (Entry k' text' tag') -> k=k' && text=text' && tag=tag')
