examples/unit-tests/format.fst
@@ -22,8 +22,12 @@ open Array
 type message = seq byte
 type msg (l:nat) = m:message{length m==l}
 
+(* ----- two lemmas on array append *) 
+
 (* Here's a small proof that append is injective. 
-   To use this property, you have to explicitly call append_inj yourself (with an implicit first arg) *)
+   To use this property, you have to explicitly call 
+   append_inj yourself (with an implicit first arg) *)
+
 val append_inj: #l:nat
                -> b1:msg l -> b2:message
                -> c1:msg l -> c2:message{append b1 b2==append c1 c2}
@@ -35,32 +39,46 @@ let rec append_inj l b1 b2 c1 c2 = match l with
 (* The same proof again, 
    But, if you give it a "Lemma" type the solver 
    will use the lemma as needed to prove other goals. *)
+
 val append_inj_lemma: b1:message -> b2:message
                    -> c1:message -> c2:message
                    -> Lemma (requires (length b1==length c1 /\ append b1 b2==append c1 c2))
                             (ensures (Equal b1 c1 /\ Equal b2 c2))
                             (decreases (length b1))
                             [SMTPat (append b1 b2); SMTPat (append c1 c2)] 
+
 let rec append_inj_lemma b1 b2 c1 c2 =
   let l = length b1 in 
   match l with
   | 0 -> ()
   | _ -> append_inj_lemma (slice b1 1 l) b2 (slice c1 1 l) c2
 
-let tag0 = create 1 0uy
-let tag1 = create 1 1uy
+
+(* ----- from strings to bytestring and back *)
 
 logic type UInt16 (i:int) = (0 <= i /\ i < 65536)
 type uint16 = i:int{UInt16 i}
 
-assume val utf8:  s:string  -> Tot (m:message{length m <= strlen s}) (* this spec is accurate for ASCII strings *)
+assume val utf8:
+  s:string  -> Tot (m:message{length m <= strlen s}) 
+  (* this spec is accurate for ASCII strings *)
+
 assume val iutf8: m:message -> s:string{utf8 s == m}
-assume UTF8_inj: forall s0 s1.{:pattern (utf8 s0); (utf8 s1)}  Equal (utf8 s0) (utf8 s1) ==> s0==s1
+
+assume UTF8_inj: 
+  forall s0 s1.{:pattern (utf8 s0); (utf8 s1)}
+    Equal (utf8 s0) (utf8 s1) ==> s0==s1
 
 assume val uint16_to_bytes: uint16 -> Tot (msg 2)
 assume UINT16_inj: forall s0 s1. Equal (uint16_to_bytes s0) (uint16_to_bytes s1) ==> s0==s1
 
 type string16 = s:string{UInt16 (length (utf8 s))} (* up to 65K *)
+
+
+(* ----- the formatting we use for authenticated RPCs *) 
+
+let tag0 = create 1 0uy
+let tag1 = create 1 1uy
 
 val request : string -> Tot message
 let request s = append tag0 (utf8 s)
@@ -71,7 +89,8 @@ let response s t =
   append tag1 (append lb (append (utf8 s) (utf8 t)))
 
 
-(* 3 lemmas on message formats: 
+(* ------- 3 lemmas on message formats: 
+
    - requests are injective on their argument
    - responses are injective on both their arguments
    - requests and responses are distinct 
@@ -80,28 +99,22 @@ let response s t =
    functions---they just return messages---so these three lemmas are
    sufficient *) 
 
-val req_resp_distinct: s:string -> s':string16 -> t':string
-                     -> Lemma (requires True)
-                              (ensures (request s <> response s' t'))
-                              [SMTPat (request s); SMTPat (response s' t')]
+val req_resp_distinct: 
+  s:string -> s':string16 -> t':string -> 
+  Lemma (requires True)
+        (ensures (request s <> response s' t'))
+        [SMTPat (request s); SMTPat (response s' t')]
 let req_resp_distinct s s' t' = ()
 
-(*
-val req_inj: s0:string -> s1:string{request s0=request s1} -> Lemma (ensures (s0==s1))
-let req_inj s0 s1 = ()
- *)
-
-val req_components_corr: s0:string
-                      -> s1:string
-                      -> Lemma (requires (request s0 == request s1))
-                               (ensures  (s0==s1))
-                               (* [SMTPat (request s0); SMTPat (request s1)] *)
+val req_components_corr: 
+  s0:string -> s1:string -> 
+  Lemma (requires (request s0 == request s1))
+        (ensures  (s0==s1))
 let req_components_corr s0 s1 = ()
 
-val resp_components_corr: s0:string16 -> t0:string 
-                       -> s1:string16 -> t1:string
-                       -> Lemma (requires (response s0 t0 == response s1 t1))
-                                (ensures  (s0==s1 /\ t0==t1))
-                                (* [SMTPat (response s0 t0); SMTPat (response s1 t1)] *)
+val resp_components_corr: 
+  s0:string16 -> t0:string -> s1:string16 -> t1:string -> 
+  Lemma (requires (response s0 t0 == response s1 t1))
+        (ensures  (s0==s1 /\ t0==t1))
 let resp_components_corr s0 t0 s1 t1 = ()
 
